theory/Mem.thy
@@ -6,15 +6,147 @@ imports
   rBPFCommType Val
 begin
 
-type_synonym mem = "(u64, u8 option) map"
+type_synonym mem = "(u64, u8) map"
+
+definition init_mem :: "mem" where
+"init_mem = (\<lambda> _. None)"
 
 datatype memory_chunk = M8 | M16 | M32 | M64
 
-type_synonym addr_type = val
+type_synonym addr_type = u64
 
+definition option_u64_of_u8_1 :: "u8 option \<Rightarrow> u64 option" where
+"option_u64_of_u8_1 v0 = (
+  case v0 of None \<Rightarrow> None |
+  Some v \<Rightarrow> Some (ucast v)
+)"
+
+definition option_u64_of_u8_2 :: "u8 option \<Rightarrow> u8 option \<Rightarrow> u64 option" where
+"option_u64_of_u8_2 v0 v1 = (
+  case v0 of None \<Rightarrow> None |
+  Some n0 \<Rightarrow> (
+    case v1 of None \<Rightarrow> None |
+    Some n1 \<Rightarrow> Some (or ((ucast n1) << 8) (ucast n0))
+  )
+)"
+
+definition option_u64_of_u8_4 :: "u8 option \<Rightarrow> u8 option \<Rightarrow> u8 option \<Rightarrow> u8 option \<Rightarrow> u64 option" where
+"option_u64_of_u8_4 v0 v1 v2 v3 = (
+  case v0 of None \<Rightarrow> None |
+  Some n0 \<Rightarrow> (
+    case v1 of None \<Rightarrow> None |
+    Some n1 \<Rightarrow> (
+      case v2 of None \<Rightarrow> None |
+      Some n2 \<Rightarrow> (
+        case v3 of None \<Rightarrow> None |
+        Some n3 \<Rightarrow>
+          Some (or ((ucast n3) << 24)
+                    (or ((ucast n2) << 16)
+                        (or ((ucast n1) << 8) (ucast n0) ) ))))
+  )
+)"
+
+definition option_u64_of_u8_8 :: "u8 option \<Rightarrow> u8 option \<Rightarrow> u8 option \<Rightarrow> u8 option \<Rightarrow>
+  u8 option \<Rightarrow> u8 option \<Rightarrow> u8 option \<Rightarrow> u8 option \<Rightarrow>  u64 option" where
+"option_u64_of_u8_8 v0 v1 v2 v3 v4 v5 v6 v7 = (
+  case v0 of None \<Rightarrow> None |
+  Some n0 \<Rightarrow> (
+    case v1 of None \<Rightarrow> None |
+    Some n1 \<Rightarrow> (
+      case v2 of None \<Rightarrow> None |
+      Some n2 \<Rightarrow> (
+        case v3 of None \<Rightarrow> None |
+        Some n3 \<Rightarrow> (
+          case v4 of None \<Rightarrow> None |
+          Some n4 \<Rightarrow> (
+            case v5 of None \<Rightarrow> None |
+            Some n5 \<Rightarrow> (
+              case v6 of None \<Rightarrow> None |
+              Some n6 \<Rightarrow> (
+                case v7 of None \<Rightarrow> None |
+                Some n7 \<Rightarrow>
+                  Some (or ((ucast n7) << 56)
+                            (or ((ucast n6) << 48)
+                              (or ((ucast n5) << 40)
+                                  (or ((ucast n4) << 32)
+                                      (or ((ucast n3) << 24)
+                                          (or ((ucast n2) << 16)
+                                              (or ((ucast n1) << 8) (ucast n0) ) ))))))))))))
+  )
+)"
+
+
+definition memory_chunk_value_of_u64 :: "memory_chunk \<Rightarrow> u64 \<Rightarrow> val" where
+"memory_chunk_value_of_u64 mc v = (
+  case mc of
+  M8 \<Rightarrow> Vbyte (ucast v) |
+  M16 \<Rightarrow> Vshort (ucast v) |
+  M32 \<Rightarrow> Vint (ucast v) |
+  M64 \<Rightarrow> Vlong (ucast v)
+)"
+
+definition option_val_of_u64 :: "memory_chunk \<Rightarrow> u64 option \<Rightarrow> val option" where
+"option_val_of_u64 mc v = (
+  case v of
+  None \<Rightarrow> None |
+  Some v1 \<Rightarrow> Some (memory_chunk_value_of_u64 mc v1)
+)"
+
+definition loadv :: "memory_chunk \<Rightarrow> mem \<Rightarrow> addr_type \<Rightarrow> val option" where
+"loadv mc m addr = ( option_val_of_u64 mc (
+  case mc of
+  M8  \<Rightarrow> option_u64_of_u8_1 (m addr) |
+  M16 \<Rightarrow> option_u64_of_u8_2 (m addr) (m (addr+1))|
+  M32 \<Rightarrow> option_u64_of_u8_4 (m addr) (m (addr+1)) (m (addr+2)) (m (addr+3))|
+  M64 \<Rightarrow> option_u64_of_u8_8 (m addr) (m (addr+1)) (m (addr+2)) (m (addr+3))
+                        (m (addr+4)) (m (addr+5)) (m (addr+6)) (m (addr+7))
+))"
+
+definition storev :: "memory_chunk \<Rightarrow> mem \<Rightarrow> addr_type \<Rightarrow> val \<Rightarrow> mem option" where
+"storev mc m addr v = (
+  case mc of
+  M8  \<Rightarrow> (
+    case v of
+    Vbyte n \<Rightarrow> Some (\<lambda> i. if i = addr then Some n else m i) |
+    _ \<Rightarrow> None) |
+  M16 \<Rightarrow> (
+    case v of
+    Vshort n \<Rightarrow>
+      let l = u8_list_of_u16 n in
+        Some (\<lambda> i. if i = addr    then Some (l!(0)) else
+                   if i = addr+1  then Some (l!(1)) else
+                      m i) |
+    _ \<Rightarrow> None) |
+  M32 \<Rightarrow> (
+    case v of
+    Vint n \<Rightarrow>
+      let l = u8_list_of_u32 n in
+        Some (\<lambda> i. if i = addr    then Some (l!(0)) else
+                   if i = addr+1  then Some (l!(1)) else
+                   if i = addr+2  then Some (l!(2)) else
+                   if i = addr+3  then Some (l!(3)) else
+                      m i) |
+    _ \<Rightarrow> None) |
+  M64 \<Rightarrow> (
+    case v of
+    Vlong n \<Rightarrow>
+      let l = u8_list_of_u64 n in
+        Some (\<lambda> i. if i = addr    then Some (l!(0)) else
+                   if i = addr+1  then Some (l!(1)) else
+                   if i = addr+2  then Some (l!(2)) else
+                   if i = addr+3  then Some (l!(3)) else
+                   if i = addr+4  then Some (l!(4)) else
+                   if i = addr+5  then Some (l!(5)) else
+                   if i = addr+6  then Some (l!(6)) else
+                   if i = addr+7  then Some (l!(7)) else
+                      m i) |
+    _ \<Rightarrow> None)
+)"
+
+ (*
 axiomatization
   loadv   :: "memory_chunk \<Rightarrow> mem \<Rightarrow> addr_type \<Rightarrow> val option" and
-  storev  :: "memory_chunk \<Rightarrow> mem \<Rightarrow> addr_type \<Rightarrow> val \<Rightarrow> mem option"
+  storev  :: "memory_chunk \<Rightarrow> mem \<Rightarrow> addr_type \<Rightarrow> val \<Rightarrow> mem option"  *)
 
 definition vlong_of_memory_chunk :: "memory_chunk \<Rightarrow> val" where
 "vlong_of_memory_chunk chunk = (
@@ -24,5 +156,7 @@ definition vlong_of_memory_chunk :: "memory_chunk \<Rightarrow> val" where
   M32 \<Rightarrow> Vlong 32 |
   M64 \<Rightarrow> Vlong 64
 )"
+
+axiomatization where store_load_consistency: "storev M32 m place v = Some m' \<Longrightarrow>  loadv M32 m' place = Some v "
 
 end
